Remove duplicate full-imap stuff from StampedMap

Spec/MapSpec.s.dfy
@@ -3,34 +3,9 @@
 
 include "../lib/Base/KeyType.s.dfy"
 include "../lib/Base/SequencesLite.s.dfy"
-include "Message.s.dfy"
+include "FullKMMap.s.dfy"
 include "AtomicStateMachine.s.dfy"
 include "CrashTolerant.s.dfy"
-
-module FullKMMapMod {
-  import opened ValueMessage
-  import opened KeyType
-  // Defines a fully-populated Key-Message imap
-
-  predicate AnyKey<K>(k: K) { true }
-  predicate Defined(kvm: imap<Key, Message>, k: Key) {
-    k in kvm && kvm[k].Define?
-  }
-  predicate KMMapIsFull(kvm: imap<Key, Message>) {
-    forall k | AnyKey(k) :: Defined(kvm, k)
-  }
-  function EmptyKMMap() : imap<Key, Message>
-    ensures KMMapIsFull(EmptyKMMap())
-  {
-    imap k | AnyKey(k) :: DefaultMessage()
-  }
-
-  // Dafny demands a compilable witness for FullKMMap, but also doesn't
-  // compile imaps. Lucky we're in a .s file so I can just lie with an
-  // axiom. This makes me feel uncomfortable.
-  function method Witness() : imap<Key,Message> ensures Witness() == EmptyKMMap()
-  type FullKMMap = ikv: imap<Key,Message> | KMMapIsFull(ikv) witness Witness()
-}
 
 module MapSpecMod refines AtomicStateMachineMod {
   import opened ValueMessage
