Splinter/CoordinationLayer/StampedMap.i.dfy
@@ -4,52 +4,21 @@
 include "../../lib/Lang/NativeTypes.s.dfy"
 include "../../lib/Base/KeyType.s.dfy"
 include "../../Spec/Message.s.dfy"
+include "../../Spec/FullKMMap.s.dfy"
 
 // A "StampedMap" is a full imap "stamped" with an LSN that identifies how many
 // operations it represents.
 module StampedMapMod {
   import opened ValueMessage
   import opened KeyType
+  import opened FullKMMapMod
 
   type LSN = nat // Log sequence number
 
-  // Provide a Triggerable symbol for the quantifier
-  predicate AnyKey(k: Key) { true }
-
-  // TODO(jonh): Okay, LSNs don't really need to be in the spec, do they?
-  datatype RawStampedMap = RawStampedMap(mi: imap<Key, Message>, seqEnd: LSN)
-  {
-    predicate secretWF() {
-      // TODO How is ImapComplete not in Maps.i?
-      // Ensures that all messages are terimal in the interp map (aka not deltas)
-      && (forall k | AnyKey(k) :: k in mi && mi[k].Define?)
-    }
-
-    // The effect of a put
-    function Put(key: Key, value: Message) : (outStampedMap : StampedMap)
-      requires value.Define?
-      requires secretWF()
-      ensures outStampedMap.secretWF()
-    {
-      RawStampedMap(mi[key := value], seqEnd + 1)
-    }
-  }
-
-  function RawEmpty() : RawStampedMap
-  {
-    RawStampedMap(imap k | AnyKey(k) :: DefaultMessage(), 0)
-  }
-
-  // Dafny demands a compilable witness for RawStampedMap, but also doesn't
-  // compile imaps. Lucky we're in a .s file so I can just lie with an
-  // axiom. This makes me feel uncomfortable.
-  function method Witness() : RawStampedMap
-    ensures Witness() == RawEmpty()
-
-  type StampedMap = ri:RawStampedMap | ri.secretWF() witness Witness()
+  datatype StampedMap = StampedMap(mi: FullKMMap, seqEnd: LSN)
 
   function Empty() : StampedMap
   {
-    RawEmpty()
+    StampedMap(EmptyKMMap(), 0)
   }
 }
