Spec/FullKMMap.s.dfy
@@ -1,0 +1,30 @@
+// Copyright 2018-2021 VMware, Inc., Microsoft Inc., Carnegie Mellon University, ETH Zurich, and University of Washington
+// SPDX-License-Identifier: BSD-2-Clause
+
+include "../lib/Base/KeyType.s.dfy"
+include "Message.s.dfy"
+
+module FullKMMapMod {
+  import opened ValueMessage
+  import opened KeyType
+  // Defines a fully-populated Key-Message imap
+
+  predicate AnyKey<K>(k: K) { true }
+  predicate Defined(kvm: imap<Key, Message>, k: Key) {
+    k in kvm && kvm[k].Define?
+  }
+  predicate KMMapIsFull(kvm: imap<Key, Message>) {
+    forall k | AnyKey(k) :: Defined(kvm, k)
+  }
+  function EmptyKMMap() : imap<Key, Message>
+    ensures KMMapIsFull(EmptyKMMap())
+  {
+    imap k | AnyKey(k) :: DefaultMessage()
+  }
+
+  // Dafny demands a compilable witness for FullKMMap, but also doesn't
+  // compile imaps. Lucky we're in a .s file so I can just lie with an
+  // axiom. This makes me feel uncomfortable.
+  function method Witness() : imap<Key,Message> ensures Witness() == EmptyKMMap()
+  type FullKMMap = ikv: imap<Key,Message> | KMMapIsFull(ikv) witness Witness()
+}
